proof/crefine/AARCH64/Tcb_C.thy
@@ -533,16 +533,6 @@ lemma threadSet_ipcbuffer_invs:
   apply (wp threadSet_invs_trivial, simp_all add: inQ_def cong: conj_cong)
   done
 
-(* FIXME AARCH64 move to SR_Lemmas where the RISCV64 version is *)
-lemma canonical_address_tcb_ptr:
-  "\<lbrakk> canonical_address t; is_aligned t tcbBlockSizeBits \<rbrakk>
-   \<Longrightarrow> canonical_address (ptr_val (tcb_ptr_to_ctcb_ptr t))"
-  apply (rule canonical_address_and_maskI)
-  apply (drule canonical_address_and_maskD)
-  apply (clarsimp simp: tcb_ptr_to_ctcb_ptr_def canonical_address_range tcbBlockSizeBits_def
-                        ctcb_offset_defs and_mask_plus)
-  done
-
 lemma invokeTCB_ThreadControl_ccorres:
   notes prod.case_cong_weak[cong]
   shows
